IR.v
@@ -1,16 +1,4 @@
-Require Import Coq.Lists.List. Import ListNotations.
-Require Import Coq.Strings.String.
-Require Import Coq.Strings.Ascii.
-Require Import Coq.Strings.Byte.
-Require Import Coq.Arith.Arith.
-Require Import Coq.ZArith.ZArith.
-Require Import Coq.PArith.PArith.
-Import IfNotations.
-From Coq Require Export Lia.
-Require Import BF.Byte.
-Require Import BF.VM.
-Require Import BF.Token.
-Require Import BF.AST.
+From BF Require Import Base Byte VM Token AST.
 
 Inductive ir : Type :=
   | IRight (n : positive) (i : ir)
@@ -21,101 +9,101 @@ Inductive ir : Type :=
   | ILoop (body : ir) (i : ir)
   | IEnd.
 
-Inductive ir_execute : ir -> vm -> vm -> Prop :=
+Inductive execute : ir -> vm -> vm -> Prop :=
   | E_IRight : forall n next v v'',
-      ir_execute next (vm_move_right n v) v'' ->
-      ir_execute (IRight n next) v v''
+      execute next (VM.move_right n v) v'' ->
+      execute (IRight n next) v v''
   | E_ILeft : forall n next v v' v'',
-      vm_move_left n v = Some v' ->
-      ir_execute next v' v'' ->
-      ir_execute (ILeft n next) v v''
+      VM.move_left n v = Some v' ->
+      execute next v' v'' ->
+      execute (ILeft n next) v v''
   | E_IAdd : forall n next v v'',
-      ir_execute next (vm_add n v) v'' ->
-      ir_execute (IAdd n next) v v''
+      execute next (VM.add n v) v'' ->
+      execute (IAdd n next) v v''
   | E_IOutput : forall next v v'',
-      ir_execute next (vm_output v) v'' ->
-      ir_execute (IOutput next) v v''
+      execute next (VM.output v) v'' ->
+      execute (IOutput next) v v''
   | E_IInput : forall next v v' v'',
-      vm_input v = Some v' ->
-      ir_execute next v' v'' ->
-      ir_execute (IInput next) v v''
+      VM.input v = Some v' ->
+      execute next v' v'' ->
+      execute (IInput next) v v''
   | E_ILoop_0 : forall body next l r o i v',
-      ir_execute next (VM l x00 r o i) v' ->
-      ir_execute (ILoop body next) (VM l x00 r o i) v'
+      execute next (VM l x00 r o i) v' ->
+      execute (ILoop body next) (VM l x00 r o i) v'
   | E_ILoop : forall body next l c r o i v' v'',
       c <> x00 ->
-      ir_execute body (VM l c r o i) v' ->
-      ir_execute (ILoop body next) v' v'' ->
-      ir_execute (ILoop body next) (VM l c r o i) v''
+      execute body (VM l c r o i) v' ->
+      execute (ILoop body next) v' v'' ->
+      execute (ILoop body next) (VM l c r o i) v''
   | E_IEnd : forall v,
-      ir_execute IEnd v v.
+      execute IEnd v v.
 
-Definition ir_equiv (i1 i2 : ir) : Prop := forall v v',
-  ir_execute i1 v v' <-> ir_execute i2 v v'.
+Definition equiv (i1 i2 : ir) : Prop := forall v v',
+  execute i1 v v' <-> execute i2 v v'.
 
-Definition ir_transform_sound (trans : ir -> ir) : Prop := forall i,
-  ir_equiv i (trans i).
+Definition transform_sound (trans : ir -> ir) : Prop := forall i,
+  equiv i (trans i).
 
-Definition ir_cons_right (n : positive) (i : ir) : ir :=
+Definition cons_right (n : positive) (i : ir) : ir :=
   match i with
   | IRight m i' => IRight (m + n) i'
   | _ => IRight n i
   end.
 
-Fixpoint ir_cons_left (n : positive) (i : ir) : ir :=
+Fixpoint cons_left (n : positive) (i : ir) : ir :=
   match i with
   | ILeft m i' => ILeft (m + n) i'
   | IRight m i' => match n ?= m with
                    | Eq => i'
                    | Lt => IRight (m - n) i'
-                   | Gt => ir_cons_left (n - m) i'
+                   | Gt => cons_left (n - m) i'
                    end
   | _ => ILeft n i
   end%positive.
 
-Fixpoint ir_cons_add (n : byte) (i : ir) : ir :=
+Fixpoint cons_add (n : byte) (i : ir) : ir :=
   match i with
-  | IAdd m i' => ir_cons_add (byte_add m n) i'
+  | IAdd m i' => cons_add (Byte.add m n) i'
   | _ => IAdd n i
   end.
 
-Fixpoint ast_lower (a : ast) : ir :=
+Fixpoint lower_ast (a : ast) : ir :=
   match a with
-  | ARight a' => IRight 1 (ast_lower a')
-  | ALeft a' => ILeft 1 (ast_lower a')
-  | AInc a' => IAdd x01 (ast_lower a')
-  | ADec a' => IAdd xff (ast_lower a')
-  | AOutput a' => IOutput (ast_lower a')
-  | AInput a' => IInput (ast_lower a')
-  | ALoop body a' => ILoop (ast_lower body) (ast_lower a')
+  | ARight a' => IRight 1 (lower_ast a')
+  | ALeft a' => ILeft 1 (lower_ast a')
+  | AInc a' => IAdd x01 (lower_ast a')
+  | ADec a' => IAdd xff (lower_ast a')
+  | AOutput a' => IOutput (lower_ast a')
+  | AInput a' => IInput (lower_ast a')
+  | ALoop body a' => ILoop (lower_ast body) (lower_ast a')
   | AEnd => IEnd
   end.
 
-Fixpoint ir_raise (i : ir) : ast :=
+Fixpoint raise_ast (i : ir) : ast :=
   match i with
-  | IRight n i' => ast_cons_right n (ir_raise i')
-  | ILeft n i' => ast_cons_left n (ir_raise i')
-  | IAdd n i' => ast_cons_add n (ir_raise i')
-  | IOutput i' => AOutput (ir_raise i')
-  | IInput i' => AInput (ir_raise i')
-  | ILoop body i' => ALoop (ir_raise body) (ir_raise i')
+  | IRight n i' => AST.cons_right n (raise_ast i')
+  | ILeft n i' => AST.cons_left n (raise_ast i')
+  | IAdd n i' => AST.cons_add n (raise_ast i')
+  | IOutput i' => AOutput (raise_ast i')
+  | IInput i' => AInput (raise_ast i')
+  | ILoop body i' => ALoop (raise_ast body) (raise_ast i')
   | IEnd => AEnd
   end.
 
-Fixpoint ir_combine (i : ir) : ir :=
+Fixpoint combine (i : ir) : ir :=
   match i with
-  | IRight n i' => ir_cons_right n (ir_combine i')
-  | ILeft n i' => ir_cons_left n (ir_combine i')
-  | IAdd n i' => ir_cons_add n (ir_combine i')
-  | IOutput i' => IOutput (ir_combine i')
-  | IInput i' => IInput (ir_combine i')
-  | ILoop body i' => ILoop (ir_combine body) (ir_combine i')
+  | IRight n i' => cons_right n (combine i')
+  | ILeft n i' => cons_left n (combine i')
+  | IAdd n i' => cons_add n (combine i')
+  | IOutput i' => IOutput (combine i')
+  | IInput i' => IInput (combine i')
+  | ILoop body i' => ILoop (combine body) (combine i')
   | IEnd => IEnd
   end.
 
-Example test_ir_execute : forall a,
+Example test_execute : forall a,
   parse (lex ",>+++[-<++>]<-.") = Some a ->
-  ir_execute (ast_lower a) (vm_make [x02]) (VM [] x07 [] [x07] []).
+  execute (lower_ast a) (VM.make [x02]) (VM [] x07 [] [x07] []).
 Proof.
   intros. inversion H; subst; clear H.
   repeat (econstructor || discriminate).
@@ -123,8 +111,8 @@ Qed.
 
 Open Scope positive_scope.
 
-Theorem ir_cons_right_left_refl : forall i n,
-  ir_cons_left n (ir_cons_right n i) = i.
+Theorem cons_right_left_refl : forall i n,
+  cons_left n (cons_right n i) = i.
 Proof.
   induction i; intros; cbn;
   try (rewrite Pos.compare_refl; reflexivity).
@@ -132,15 +120,15 @@ Proof.
   f_equal. lia.
 Qed.
 
-Theorem ir_cons_right_right : forall i n m,
-  ir_cons_right m (ir_cons_right n i) = ir_cons_right (n + m) i.
+Theorem cons_right_right : forall i n m,
+  cons_right m (cons_right n i) = cons_right (n + m) i.
 Proof.
   induction i; intros; cbn; try reflexivity.
   f_equal. lia.
 Qed.
 
-Theorem ir_cons_left_left : forall i n m,
-  ir_cons_left m (ir_cons_left n i) = ir_cons_left (n + m) i.
+Theorem cons_left_left : forall i n m,
+  cons_left m (cons_left n i) = cons_left (n + m) i.
 Proof.
   induction i; intros; cbn; try (f_equal; lia).
   destruct (n0 ?= n) eqn:Hcomp1.
@@ -171,76 +159,76 @@ Qed.
 
 Close Scope positive_scope.
 
-Theorem ast_lower_sound : forall a v v',
-  ast_execute a v v' -> ir_execute (ast_lower a) v v'.
+Theorem lower_ast_sound : forall a v v',
+  AST.execute a v v' -> execute (lower_ast a) v v'.
 Proof.
   intros. induction H; cbn.
-  - apply E_IRight, IHast_execute.
-  - eapply E_ILeft. apply H. apply IHast_execute.
-  - apply E_IAdd, IHast_execute.
-  - apply E_IAdd, IHast_execute.
-  - apply E_IOutput, IHast_execute.
-  - eapply E_IInput. apply H. apply IHast_execute.
-  - apply E_ILoop_0, IHast_execute.
-  - eapply E_ILoop. apply H. apply IHast_execute1. apply IHast_execute2.
+  - apply E_IRight, IHexecute.
+  - eapply E_ILeft. apply H. apply IHexecute.
+  - apply E_IAdd, IHexecute.
+  - apply E_IAdd, IHexecute.
+  - apply E_IOutput, IHexecute.
+  - eapply E_IInput. apply H. apply IHexecute.
+  - apply E_ILoop_0, IHexecute.
+  - eapply E_ILoop. apply H. apply IHexecute1. apply IHexecute2.
   - apply E_IEnd.
 Qed.
 
-Theorem ir_execute_cons_right : forall i n v v'',
-  ir_execute (ir_cons_right n i) v v'' <->
-  ir_execute i (vm_move_right n v) v''.
+Theorem execute_cons_right : forall i n v v'',
+  execute (cons_right n i) v v'' <->
+  execute i (VM.move_right n v) v''.
 Proof.
   split.
   - induction i; intros;
     inversion H; subst; try assumption.
     apply E_IRight.
-    rewrite vm_move_right_right, Pos.add_comm. assumption.
+    rewrite VM.move_right_right, Pos.add_comm. assumption.
   - induction i; intros;
     apply E_IRight; try assumption.
     inversion H; subst.
-    rewrite vm_move_right_right, Pos.add_comm in H4. assumption.
+    rewrite VM.move_right_right, Pos.add_comm in H4. assumption.
 Qed.
 
-Theorem ir_execute_cons_left : forall i n v v' v'',
-  vm_move_left n v = Some v' ->
-  ir_execute (ir_cons_left n i) v v'' <->
-  ir_execute i v' v''.
+Theorem execute_cons_left : forall i n v v' v'',
+  VM.move_left n v = Some v' ->
+  execute (cons_left n i) v v'' <->
+  execute i v' v''.
 Proof.
   split.
   - induction i; intros; cbn in *.
-    + apply E_IRight. destruct vm_move_left; inversion H; subst.
+    + apply E_IRight. destruct VM.move_left; inversion H; subst.
 Admitted.
 
-Theorem ir_execute_cons_add : forall i n v v'',
-  ir_execute (ir_cons_add n i) v v'' <->
-  ir_execute i (vm_add n v) v''.
+Theorem execute_cons_add : forall i n v v'',
+  execute (cons_add n i) v v'' <->
+  execute i (VM.add n v) v''.
 Proof.
   split;
   generalize dependent v''; generalize dependent v; generalize dependent n.
   - induction i; intros;
     try (inversion H; subst; assumption).
-    apply E_IAdd. rewrite vm_add_add, byte_add_comm. apply IHi, H.
+    apply E_IAdd. rewrite VM.add_add, Byte.add_comm. apply IHi, H.
   - induction i; intros;
     inversion H; subst; repeat constructor; try assumption.
-    rewrite vm_add_add, byte_add_comm in H4. apply IHi, H4.
+    rewrite VM.add_add, Byte.add_comm in H4. apply IHi, H4.
 Qed.
 
-Theorem ir_combine_sound :
-  ir_transform_sound ir_combine.
+Theorem combine_sound :
+  transform_sound combine.
 Proof.
-  unfold ir_transform_sound, ir_equiv.
+  unfold transform_sound, equiv.
   split.
   - intros. induction H; cbn;
     try (econstructor; eassumption).
-    + rewrite ir_execute_cons_right; assumption.
-    + rewrite ir_execute_cons_left; eassumption.
-    + rewrite ir_execute_cons_add; assumption.
+    + rewrite execute_cons_right; assumption.
+    + rewrite execute_cons_left; eassumption.
+    + rewrite execute_cons_add; assumption.
   - generalize dependent v'; generalize dependent v.
     induction i; intros; cbn in *.
-    + rewrite ir_execute_cons_right in H. apply E_IRight, IHi, H.
-    + rewrite ir_execute_cons_left in H. eapply E_ILeft.
+    + rewrite execute_cons_right in H. apply E_IRight, IHi, H.
+    + rewrite execute_cons_left in H. eapply E_ILeft.
       admit. apply IHi. eassumption. admit.
-    + rewrite ir_execute_cons_add in H. apply E_IAdd, IHi, H.
+    + rewrite execute_cons_add in H. apply E_IAdd, IHi, H.
     + inversion H; subst. apply E_IOutput, IHi, H1.
     + inversion H; subst. eapply E_IInput. admit. apply IHi, H2.
     + inversion H; subst.
